

\section{Theories\label{apx:math}}
%----------------------------------------------------------------

%-----------------------------------------------------------------------------
	\subsection{Basic\_Function\_Properties\_Theory}	%-----------------------------------------------------------------------------

\begin{lstlisting}[language=resolve]
Theory Basic_Function_Properties_Theory;
		uses Boolean_Theory;

	Implicit Definition Is_Injective(F : (D : MType) -> (R : MType)) : B is
		For all d1, d2 : D,
			F(d1) = F(d2) implies d1 = d2;

end;
\end{lstlisting}

%-----------------------------------------------------------------------------
	\subsection{Binary\_Iterator\_Theory}	%-----------------------------------------------------------------------------

\begin{lstlisting}[language=resolve]
Precis Binary_Iterator_Theory;
		uses Integer_Theory, String_Theory, Conditional_Function_Theory;

	Definition Iterative_Apply(Step : ((R : MType) * (V : MType)) -> R,
		Start : R, Value_Function : Z -> V, Value_Count : Z) : R;

	Definition Concatenate(Value_Function : Z -> (T : MType), 
			Value_Count : Z) : Str(T) = 
		Iterative_Apply(lambda (s : Str(T), t : T).(s o <t>),
			Empty_String, Value_Function, Value_Count);

	Definition Shift(Value_Function : Z -> (V : MType), offset : Z) : 
		Z -> V;

	Theorem Concatenation_Length:
		For all f : Z -> Entity,
		For all i : Z,
			|Concatenate(f, i)| = i;

	Theorem Zero_Length_Concatenate:
		For all f : Z -> Entity,
			Concatenate(f, 0) = Empty_String;

	Theorem End_Changed:
		For all f : Z -> Entity,
		For all e : Entity,
		For all i : Z,
			Concatenate(
				lambda (j : Z).({{
					e if j = i;
					f(j) otherwise;
				}}),
				i)
			= Concatenate(f, i - 1) o <e>;

	Theorem End_Excluded:
		For all f : Z -> Entity,
		For all e : Entity,
		For all i : Z,
			Concatenate(
				lambda (j : Z).({{
					e if j = i;
					f(j) otherwise;
				}}),
				i - 1)
			= Concatenate(f, i - 1);

	Theorem Inductive_Reverse_1:
		For all f : Z -> Entity,
		For all i : Z,
		Reverse(Concatenate(f, i)) = 
			<f(i)> o Reverse(Concatenate(f, i - 1));
end;
\end{lstlisting}

%-----------------------------------------------------------------------------
	\subsection{Binary\_Relation\_Properties\_Theory}	%-----------------------------------------------------------------------------

\begin{lstlisting}[language=resolve]
Precis Binary_Relation_Properties_Theory;
		uses Boolean_Theory;

	Definition Is_Antisymmetric(f : (Entity * Entity) -> B) : B;

	Theorem Antisymmetric_Implies_Equal:
		For all f : (Entity * Entity) -> B,
		For all a, b : Entity,
			Is_Antisymmetric(f) implies 
				((f(a, b) and f(b, a)) = (a = b));

end;

\end{lstlisting}

%-----------------------------------------------------------------------------
	\subsection{Integer\_Theory}	%-----------------------------------------------------------------------------

\begin{lstlisting}[language=resolve]
Precis Integer_Theory;
    uses Boolean_Theory, Set_Theory, Monogenerator_Theory;

	(* Note that the type Z is built-in.  No need to introduce it here.
	 * As a demonstration of how we might do so, however, we introduce the
	 * type ZZ, which is isomorphic to Z. *)

	Categorical Definition introduces
		ZZ : MType, ZZ0 : ZZ, succ : ZZ -> ZZ
	related by
		Is_Monogenerator_For(ZZ, ZZ0, succ);

	Definition N : Powerset(Z);

	Definition 0: N;
	Definition 1: N;
	Definition 2: N;

	Definition z : Z;

	Type Theorem N_Subset_of_Z:
		For all n : N,
			n : Z;

	Definition TakesZs(zs : (Z * Z * Z)) : B;
	Definition SomeNs : (N * N * N);
	Definition AFact : B = TakesZs(SomeNs);

    Definition neg: Z -> Z;

    Definition suc: Z -> Z;

    --------------------------------------------------------------

    Definition (i: Z) + (j: Z): Z = 0;

    Definition (i: Z) - (j: Z): Z = 0;

    Definition (i: Z) * (j: Z) : Z = 0;

    Definition (i: Z) ** (j: Z) : Z = 0;

    Definition (i: Z) / (j: Z) : Z = 0;

    Definition (i: Z) mod (j: Z) : Z = 0;

    Definition (i: Z) rem (j: Z) : Z = 0;

    Definition (i: Z) div (j: Z) : Z = 0;

    Definition (i: Z) <= (j: Z) : B = true;

    Definition (i: Z) >= (j: Z) : B = true;

    Definition (i: Z) < (j: Z) : B = true;

    Definition (i: Z) > (j: Z) : B = true;

    Definition |(i: Z)| : Z = 0;

    Definition (i: Z) .. (j: Z) : Set(Z) = Empty_Set;

	Definition Sum(a : Z, s : Set(Z)) : Z;

    Definition Summation(s: Set(Z), f: Z -> Z) : Z = 0;

	Definition isEven(i : Z) : B = true;

	---------------------------------------------------------------
	-- Obvious Theorems                                          --
	---------------------------------------------------------------
	Theorem Zero_Less_Than_One: 0 < 1;
	Theorem One_Greater_Than_Zero: 1 > 0;
	Theorem Two_Greater_Than_Zero: 2 > 0;

	Theorem Zero_Not_Equal_To_Two: 2 /= 0;

	---------------------------------------------------------------
	-- Relation Theorems                                         --
	---------------------------------------------------------------

	Theorem Negation_1:
		For all i, j : Z,
			not(i <= j) = (i > j);

	Theorem NN_Not_Greater_Than_Zero:
		For all n : N,
			not(n > 0) = (n = 0);

	Theorem NN_Not_Zero_Addition_Right_LET:
		For all n, m : N, 
		For all i : Z,
			n + m <= i and m /= 0 implies n < i;

	Theorem NN_Not_Zero_Addition_Left_LET:
		For all n, m : N, 
		For all i : Z,
			n + m <= i and n /= 0 implies m < i;

	Theorem Even_More_LT_1:
		For all i, j, k : Z,
			i + j <= k and j > 0 implies i < k;

	Theorem Even_More_LT_2:
		For all i, j, k : Z,
			i + j <= k and i > 0 implies j < k;

	Theorem Greater_Than_Zero_Not_Equal_Zero:
		For all i : Z,
			i > 0 implies i /= 0;

	Theorem Not_Equal_Syntax:
		For all i, j : Z,
			not(i = j) = (i /= j);

	Theorem GET_And_Not_Equal_GT:
		For all i, j : Z,
			(i >= j and i /= j) = (i > j);

	Theorem Bound_1_1:
		For all i, j : Z,
			(i + 1 <= j) = (i < j);

	Theorem Bound_1_2:
		For all i, j : Z,
			(i <= j - 1) = (i < j);

	Theorem Bound_1_3:
		For all i, j : Z,
			(i - 1 >= j) = (i > j);

	Theorem Bound_N_1:
		For all i, j, k : Z,
			(i + j <= k) and j >= 0 implies i <= k;

	Theorem Bound_N_2:
		For all i, j, k : Z,
			(i <= j) and (0 <= k) implies (i <= j + k);

	Theorem Bound_N_3:
		For all i, j, k : Z,
			0 <= k implies i - ((j + k) + 1) < i - j;

	Theorem Thingy:
		For all i, j : Z,
			0 <= i implies i + 1 > 0;

	Theorem Div2_Maintains_Parity:
		For all i : Z,
			0 <= i implies 0 <= i / 2;

	Theorem Approach_By_Half_1:
		For all i, j, k : Z,
			i <= k and j <= k implies i + (j - i) / 2 <= k; 

	Theorem Half_LET_If_Positive:
		For all i : Z,
			0 <= i implies i / 2 <= i;

	Theorem Balance:
		For all i, j, k : Z,
			(i + k) + (j - k) = (i + j);

	Theorem Easy_Less_Than:
		For all i : Z,
			i - 1 < i;

	Theorem LET_Both:
		For all i, j, k : Z,
			i <= j and k > j implies i < k;

	Theorem Less_Than_Equal_Self:
		For all i : Z,
			i <= i;

	Theorem Switch_1:
		For all i, j : Z,
			(i > j) = (j < i);

	Theorem Switch_2:
		For all i, j : Z,
			(i >= j) = (j <= i);

	Theorem Weaken_1:
		For all i, j : Z,
			i > j implies i >= j;

	Theorem Weaken_2:
		For all i, j : Z,
			i < j implies i <= j;

	Theorem LET_Transitive:
		For all i, j, k : Z,
			i <= j and j <= k implies i <= k;

	Theorem Mixed_Transitive_1:
		For all i, j, k : Z,
			i < j and j <= k implies i < k;

	Theorem Off_by_One_1:
		For all i, j : Z,
			(i <= j) = (i < j + 1);

	Theorem Off_by_One_2:
		For all i, j : Z,
			(i < j) = (i + 1 <= j);

	Theorem Off_by_One_3:
		For all i, j : Z,
			(i < j) = (i <= j - 1);

	Theorem Off_by_One_4:
		For all i, j : Z,
			(i - 1 < j) = (i <= j);

	Theorem Off_by_One_5:
		For all i, j : Z,
			(i > j) = (i - 1 >= j);

	Theorem Subtract_One_from_both_LET:
		For all i, j : Z,
			(i <= j) = ((i - 1) <= (j - 1));

	Theorem LET_Subtract_One_Still_Less:
		For all i, j : Z,
			i <= j implies i - 1 <= j;

	Theorem Add_One_Still_More:
		For all i, j : Z,
			i <= j implies i <= j + 1;

	Theorem Subtract_Positive_Still_Less:
		For all i, j, k : Z,
			i <= j and k >= 0 implies i - k <= j;

	Theorem LET_But_Not_Equal_1:
		For all i, j : Z,
			(i <= j and j /= i) = (i < j);

	Theorem Cheap_LEQ_Theorem_1:
		For all i, j, k : Z,
			k <= j and i <= 0 implies i <= j - k;

	Theorem Subtact_Makes_Less:
		For all i, j, k : Z,
			i = j - k and k > 0 implies i < j;

	---------------------------------------------------------------
	-- Zero Theorems                                             --
	---------------------------------------------------------------

	Theorem Zero_Property_Right:
		For all i : Z,
			i + 0 = i;

	Theorem Zero_Property_Left:
		For all i : Z,
			0 + i = i;

	Theorem Zero_Minus_Property:
		For all i : Z,
			i - 0 = i;

	Theorem Zero_Multiplication_Right:
		For all i : Z,
			i * 0 = 0;

	Theorem Zero_Multiplication_Left:
		For all i : Z,
			0 * i = 0;

	---------------------------------------------------------------
	-- Arithmetic                                                --
	---------------------------------------------------------------

	Theorem Plus_Minus:
		For all i, j : Z,
			i + j - j = i;

	Theorem Minus_Itself_1:
		For all i : Z,
			i - i = 0;

	Theorem Minus_Itself_2:
		For all i, j : Z,
			i - (i + j) = -j;

	Theorem Subtract_Both_Sides_LET:
		For all i, j : Z,
			(i <= j) = (0 <= j - i);

	Theorem Equality_Move_Subtraction_1:
		For all i, j, k : Z,
			(i = j - k) = (i + k = j);

	Theorem LET_Move_Subtraction_1:
		For all i, j, k : Z,
			(i <= j + k) = (i - k <= j);

	Theorem Distribute_Minus_1:
		For all i, j, k : Z,
			(i - (j - k)) = (i - j + k);

	Theorem Distribute_Mult_1:
		For all i , j : Z,
			(i * (j + 1)) = (i * j) + i;

	Theorem Multiplication_Identity_1:
		For all i : Z,
			i * 1 = i;

	Theorem Multiplication_Identity_2:
		For all i : Z,
			1 * i = i;

	Theorem EI_Test:
		For all i, j, k : Z,
			i <= j / 2 and
			k >= j implies
				i <= k / 2;

	Theorem Plus_Inverse:
		For all i : Z,
			-i + i = 0;

	Theorem Plus_Associative:
		For all i, j, k : Z,
			((i + j) + k) = (i + (j + k)); 

	Theorem Cancel_Term_1:
		For all i, j, k : Z,
			i + j - k - i = j - k;

end;
\end{lstlisting}

%-----------------------------------------------------------------------------
	\subsection{Monogenerator\_Theory}	%-----------------------------------------------------------------------------

\begin{lstlisting}[language=resolve]
Precis Monogenerator_Theory;
		uses Basic_Function_Properties_Theory;

	Implicit Definition Is_Monogenerator_For(
		T : MType, Start : T, F : T -> T) : B
	is
		(For all t : T, F(t) /= t) and
		(Is_Injective(F)) and
		(For all T2 : Powerset(T),
			Instance_Of(T2, Start) and 
			(for all t : T, 
					Instance_Of(T2, t) 
						implies Instance_Of(T2, F(t)))
				implies T2 = T);

end;
\end{lstlisting}

%-----------------------------------------------------------------------------
	\subsection{Set\_Theory}	%-----------------------------------------------------------------------------

\begin{lstlisting}[language=resolve]
Precis Set_Theory;
    uses Boolean_Theory;

	Definition Set : (MType -> Powerset(SSet));

	Type Theorem Restricted_Set_Subtype_of_Big_Set:
		For all T : MType,
		For all S : Set(T),
			S : SSet;

	Type Theorem Empty_Set_In_All_Sets:
		For all T : MType,
			Empty_Set : Set(T);

	Definition Is_In(e : Entity, T : MType) : B;

end;

\end{lstlisting}

%-----------------------------------------------------------------------------
	\subsection{String\_Theory}	%-----------------------------------------------------------------------------

\begin{lstlisting}[language=resolve]
Precis String_Theory;
    uses Integer_Theory;

	--The type of all strings of heterogenous type
	Definition SStr : MType;
	Definition Empty_String : SStr;

	--A function that restricts SStr to the type of all strings of some homogenous
	--type
	Definition Str : MType -> MType;
	Definition Empty_String_In(T : MType) : Str(T);

	Type Theorem Empty_String_In_All_Strs:
		For all T : MType,
			Empty_String : Str(T);

	Type Theorem All_Strs_In_SStr:
		For all T : MType,
		For all S : Str(T),
			S : SStr;

	--If R is a subset of T, then Str(R) is a subset of Str(T)
	Type Theorem Str_Subsets:
		For all T : MType,
		For all R : Powerset(T),
		For all s : Str(R),
			s : Str(T);

	--String length
	Definition |(s : SStr)| : N;

	--String concatenation
	--Definition (s : Str(U : MType)) o (t : Str(U)) : Str(U);
	Definition (s : SStr) o (t : SStr) : SStr;

	Type Theorem Concatenation_Preserves_Generic_Type:
		For all T : MType,
		For all U, V : Str(T),
			U o V : Str(T);

	--Definition Reverse(s : Str(U : MType)) : Str(U);

	Definition Reverse(s : SStr) : SStr;

	Type Theorem Reverse_Preserves_Generic_Type:
		For all T : MType,
		For all S : Str(T),
			Reverse(S) : Str(T);

	--Singleton string
	Definition <(e : (U : MType))> : Str(U);

	Definition Is_Permutation(s : SStr, t : SStr) : B;

	--Determines if for every pairing of elements from s and t, the given predicate
	--holds
	Definition Is_Universally_Related(s : SStr, t : SStr, 
		f : (Entity * Entity) -> B) : B;

	Definition Substring(s : Str(U : MType), startInclusive : Z, length : Z) :
		Str(U);

	Definition Element_At(i : Z, s : SStr) : Entity;

	Type Theorem Element_At_Extracts_Generic_Type:
		For all T : MType,
		For all S : Str(T),
		For all i : Z,
			Element_At(i, S) : Str(T);

	Definition Exists_Between(E : Entity, S : SStr, From : Z, To : Z) : B;

	---------------------------------------------------------------
	-- Empty String Theorems                                     --
	---------------------------------------------------------------
	Theorem Reverse_Empty_String:
		Reverse(Empty_String) = Empty_String;

	Theorem Empty_String_Concatenation_Right:
		For all S : SStr,
			S o Empty_String = S;

	Theorem Empty_String_Concatenation_Left:
		For all S : SStr,
			Empty_String o S = S;

	---------------------------------------------------------------
	-- String Length Theorems                                    --
	---------------------------------------------------------------
	Theorem Same_String_Same_Length:
		For all S, T : SStr,
			S = T implies |S| = |T|;

	Theorem String_Length_Boundary_1:
		For all S, T : SStr,
		For all i : Z,
			|S o T| <= i implies
				|S| <= i and
				|T| <= i;

	Theorem String_Length_Boundary_2:
		For all S, T : SStr,
		For all i : Z,
			|S o T| < i implies
				|S| < i and
				|T| < i;

	Theorem Lenght_Concatenate_Singleton:
		For all S : SStr,
		For all e : Entity,
			|S o <e>| = |S| + 1;

	Theorem String_Length_Boundary_Singleton_Left:
		For all S : SStr,
		For all E : Entity,
		For all i : Z,
			|<E> o S| <= i implies
				|S| < i;

	Theorem String_Length_Hack_1:
		For all U, V : SStr,
		For all E : Entity,
		For all i : Z,
			|U o (<E> o V)| <= i implies
				|U| < i and
				|V| < i;

	Theorem Reverse_Irrelevant_In_Length:
		For all S : SStr,
			|Reverse(S)| = |S|;

	Theorem Concatenate_Singleton_Increases_Length_Left:
		For all S : SStr,
		For all E : Entity,
			(|S| < |<E> o S|);

	Theorem Concatenate_Singleton_Increases_Length_Right:
		For all S : SStr,
		For all E : Entity,
			(|S| < |S o <E>|);

	Theorem Zero_Length_Implies_Empty_String:
		For all S : SStr,
			(|S| = 0) = (S = Empty_String);

	Theorem Length_Concatenation:
		For all U, V : SStr,
			|U o V| = |U| + |V|;

	Theorem Get_Rid_Of_Singleton_1:
		For all S, T : SStr,
		For all e : Entity,
			(|S o <e>| = |T|) implies
				(|S| < |T|);

	Theorem Get_Rid_Of_Singleton_2:
		For all S, T : SStr,
		For all e : Entity,
			(|<e> o S| = |T|) implies
				(|S| < |T|);

	Theorem Length_Relation_1:
		For all S, T, U : SStr,
			|S o T| = |U| and |S| > 0 implies
				|T| < |U|;

	Theorem Length_Relation_2:
		For all S : SStr,
		For all e : Entity,
		For all i, j : Z,
			|S o <e>| = i and i <= j implies |S| < j;

	---------------------------------------------------------------
	-- Singleton String Theorems                                 --
	---------------------------------------------------------------
	Theorem Reverse_Of_Singleton:
		For all E : Entity,
			Reverse(<E>) = <E>;

	---------------------------------------------------------------
	-- Reverse Theorems                                          --
	---------------------------------------------------------------
	Theorem Concatenation_Under_Reverse:
		For all U, V : SStr,
			Reverse(U o V) = Reverse(V) o Reverse(U);

	Theorem Reverse_Inverts_Itself:
		For all S : SStr,
			Reverse(Reverse(S)) = S;

	---------------------------------------------------------------
	-- Concatenation Theorems                                    --
	---------------------------------------------------------------
	Theorem Concatenation_Associative:
		For all U, V, W : SStr,
			(U o V) o W = U o (V o W);

	---------------------------------------------------------------
	-- Permutation Theorems                                      --
	---------------------------------------------------------------
	Theorem Identity_Permutation:
		For all S : SStr,
			Is_Permutation(S, S);

	Theorem Permutation_Lengths:
		For all S, T : SStr,
			Is_Permutation(S, T) implies |S| = |T|;

	Theorem Permutation_Extension_1:
		For all S, T, U, V : SStr,
			Is_Permutation(S, T) and
			Is_Permutation(T o U, V) implies
				Is_Permutation(S o U, V);

	Theorem Permutation_Shell_Game_1:
		For all S, T, U, V : SStr,
			Is_Permutation(S o (T o U), V) =
				Is_Permutation((S o U) o T, V);

	Theorem Permutation_Shell_Game_2:
		For all S, T : SStr,
			Is_Permutation(S o T, T o S);

	Theorem Permutation_Shell_Game_3:
		For all S, T, U, V, W : SStr,
			Is_Permutation((S o (T o U)) o V, W) =
				Is_Permutation(((S o V) o U) o T, W);

	Theorem Permutation_Commutative:
		For all S, T : SStr,
			Is_Permutation(S, T) = Is_Permutation(T, S);

	---------------------------------------------------------------
	-- Universal Relations Theorems                              --
	---------------------------------------------------------------
	Theorem Empty_String_Universally_Related_1:
		For all S : SStr,
		For all f : (Entity * Entity) -> B,
			Is_Universally_Related(Empty_String, S, f);

	Theorem Empty_String_Universally_Related_2:
		For all S : SStr,
		For all f : (Entity * Entity) -> B,
			Is_Universally_Related(S, Empty_String, f);

	Theorem Universally_Related_Distributes_1:
		For all f : (Entity * Entity) -> B,
		For all S, T, U : SStr,
			Is_Universally_Related(S o T, U, f) implies
				Is_Universally_Related(S, U, f) and
				Is_Universally_Related(T, U, f);

	Theorem Universally_Related_Distributes_2:
		For all f : (Entity * Entity) -> B,
		For all S, T, U : SStr,
			Is_Universally_Related(S, T o U, f) implies
				Is_Universally_Related(S, T, f) and
				Is_Universally_Related(S, U, f);

	Theorem Universally_Related_Distributes_3:
		For all f : (Entity * Entity) -> B,
		For all S, T, U : SStr,
			Is_Universally_Related(S, U, f) and
			Is_Universally_Related(T, U, f) implies
				Is_Universally_Related(S o T, U, f);

	Theorem Universally_Related_Distributes_4:
		For all f : (Entity * Entity) -> B,
		For all S, T, U : SStr,
			Is_Universally_Related(S, T, f) and
			Is_Universally_Related(S, U, f) implies
				Is_Universally_Related(S, T o U, f);

	Theorem Permutation_Maintains_Universal_Relation_1:
		For all f : (Entity * Entity) -> B,
		For all S, T, U : SStr,
			Is_Universally_Related(S, T, f) and
			Is_Permutation(U, T) implies
				Is_Universally_Related(S, U, f);

	Theorem Permutation_Maintains_Universal_Relation_2:
		For all f : (Entity * Entity) -> B,
		For all S, T, U : SStr,
			Is_Universally_Related(S, T, f) and
			Is_Permutation(U, S) implies
				Is_Universally_Related(U, T, f);

	Theorem Universal_Relation_Transitivity_1:
		For all f : (Entity * Entity) -> B,
		For all S : SStr,
		For all e1, e2 : Entity,
			f(e1, e2) and Is_Universally_Related(<e2>, S, f) implies
				Is_Universally_Related(<e1>, S, f);

	Theorem Universally_Related_Singletons:
		For all e1, e2 : Entity,
		For all f : (Entity * Entity) -> B,
			f(e1, e2) = Is_Universally_Related(<e1>, <e2>, f);

	---------------------------------------------------------------
	-- Exists_Between Theorems                                   --
	---------------------------------------------------------------
	Theorem Exists_Between_No_Window_1:
		For all e : Entity,
		For all S : SStr,
		For all i : Z,
			Exists_Between(e, S, i, i - 1) = false;

	Theorem Exists_Between_No_Window_2:
		For all e : Entity,
		For all S : SStr,
		For all i : Z,
			Exists_Between(e, S, i + 1, i) = false;

	Theorem Exists_Between_Decomposition:
		For all e : Entity,
		For all S : SStr,
		For all i, j, x, y : Z,
			x >= y - 1 implies
				((Exists_Between(e, S, i, x) or
				Exists_Between(e, S, y, j)) =
					Exists_Between(e, S, i, j));
end;

\end{lstlisting}

%-----------------------------------------------------------------------------
	\subsection{Total\_Preordering\_Theory}	%-----------------------------------------------------------------------------

\begin{lstlisting}[language=resolve]
Theory Total_Preordering_Theory;
		uses String_Theory;

	Definition Is_Total_Preordering(f : ((D : MType) * D) -> B) : B =
		(For all d1 : D, f(d1, d1)) and
		(For all d1, d2, d3 : D, f(d1, d2) and f(d2, d3) 
			implies f(d1, d3)) and
		(For all d1, d2 : D, f(d1, d2) or f(d2, d1));		

	Definition Is_Conformal_With(f : (Entity * Entity) -> B, S : SStr) : B =
		For all i, j : Z,
			1 <= i and i <= j and j <= |S| implies
				f(Element_At(i, S), Element_At(j, S));

	---------------------------------------------------------------
	-- Conformity Theorems                                       --
	---------------------------------------------------------------
	Theorem Empty_String_Conformal:
		For all f : (Entity * Entity) -> B,
			Is_Conformal_With(f, Empty_String);

	Theorem Conformal_String_Extension:
		For all f : (Entity * Entity) -> B,
		For all S : SStr,
		For all e : Entity,
			Is_Conformal_With(f, S) and
			Is_Universally_Related(S, <e>, f)
				implies Is_Conformal_With(f, S o <e>);

	Theorem Total_Preordering_Symmetric:
		For all f : (Entity * Entity) -> B,
		For all e1, e2 : Entity,
			Is_Total_Preordering(f) and
			f(e1, e2) = not(f(e2, e1));

	---------------------------------------------------------------
	-- Relation Theorems                                         --
	---------------------------------------------------------------
	Theorem Symmetric_Theorem:
		For all f : (Entity * Entity) -> B,
		For all e1, e2 : Entity,
			Is_Total_Preordering(f) and not(f(e1, e2)) implies
				f(e2, e1);
end;
\end{lstlisting}
